\documentclass[12pt]{article}
\usepackage[utf8]{inputenc}
\usepackage{amsmath}
\usepackage{amsfonts}
\usepackage{amssymb}
\usepackage{amsthm}
\usepackage{mathrsfs}
\usepackage{bm}

\newenvironment{sol}
  {\par\vspace{3mm}\noindent{\it Solution}.}
  {\qed}

\begin{document}
\author{Chen Cheng, 1130339005}
\title{Homework of Chapter 8}
\maketitle
%% 8.1
\begin{flushleft}
\textbf{Ex. 8.1}
\end{flushleft}

\begin{sol}
Since log function is a strictly concave function. Using Jensen's inequality, we have
\begin{equation*}
\begin{split}
&E_qlog[r(Y)/q(Y)]\\
\leq&logE_q[r(Y)/q(Y)]\\
=&log\int[r(y)/q(y)]q(y)\mathrm{d}y\\
=&log\int r(y)\mathrm{d}y\\
=&log 1\\
=&0\\
\end{split}
\end{equation*}
The Jensen's equality shows that $E_qlog[r(Y)/q(Y)]$ is maximized as a function of $r(y)$ when $r(y)=q(y)$.\\
According to the definition of (8.46), we have
\begin{equation*}
\begin{split}
R(\theta',\theta)=&E[\ell_1(\theta',\mathbf{Z}^M|\mathbf{Z})|\mathbf{Z},\theta]\\
=&E[logPr(\mathbf{Z}^M|\mathbf{Z},\theta')|\mathbf{Z},\theta]\\
R(\theta,\theta)=&E[\ell_1(\theta,\mathbf{Z}^M|\mathbf{Z})|\mathbf{Z},\theta]\\
=&E[logPr(\mathbf{Z}^M|\mathbf{Z},\theta)|\mathbf{Z},\theta]\\
\end{split}
\end{equation*}
Then, using the equality we have just proved above, we can get
\begin{equation*}
\begin{split}
R(\theta',\theta)-R(\theta,\theta)=
&E[logPr(\mathbf{Z}^M|\mathbf{Z},\theta')|\mathbf{Z},\theta]-E[logPr(\mathbf{Z}^M|\mathbf{Z},\theta)|\mathbf{Z},\theta]\\
=&E[log(Pr(\mathbf{Z}^M|\mathbf{Z},\theta')/Pr(\mathbf{Z}^M|\mathbf{Z},\theta))|\mathbf{Z},\theta]\\
&\leq0\\
\end{split}
\end{equation*}
Thus, we have proved $R(\theta,\theta)\geq R(\theta',\theta)$.\\
\end{sol}

%% 8.3
\def \Ult {U_\ell^{(t)}}
\def \ult {u_\ell^{(t)}}
\begin{flushleft}
\textbf{Ex. 8.3}
\end{flushleft}

\begin{sol}
\begin{equation*}
\begin{split}
&E_{\Ult}[Pr(u|\Ult,\ell\neq k)]\\
=&\int Pr(u|\ult,\ell\neq k)Pr(\ult,\ell\neq k)\mathrm{d}\ell\neq k\\
=&Pr_{U_k}(u)\\
\end{split}
\end{equation*}
So, we have
\begin{equation*}
\begin{split}
E[\hat{Pr}_{U_k}(u)]=&E[\frac{1}{M-m+1}\sum_{t=m}^MPr(u|\Ult,\ell\neq k)]\\
=&\frac{1}{M-m+1}\sum_{t=m}^ME[Pr(u|\Ult,\ell\neq k)]\\
=&Pr_{U_k}(u)\\
\end{split}
\end{equation*}
Thus, we have justified the estimate (8.50).\\
\end{sol}
\end{document}